tests/lean/run/471.lean
@@ -1,0 +1,29 @@
+inductive vec : Nat → Type where
+  | nil : vec 0
+  | cons : Int → vec n → vec n.succ
+
+def vec_len : vec n → Nat
+  | vec.nil => 0
+  | x@(vec.cons h t) => vec_len t + 1
+
+def vec_len' : {n : Nat} → vec n → Nat
+  | _, vec.nil => 0
+  | _, x@(vec.cons h t) => vec_len' t + 1
+
+def tst1 : vec (n+1) → Int × vec (n+1) × vec n
+  | x@(vec.cons h t) => (h, x, t)
+
+def tst2 : vec n → Option (Int × vec n)
+  | x@(vec.cons h t) => some (h, x)
+  | _ => none
+
+example (a : Int) (x : vec n) : tst2 (vec.cons a x) = some (a, vec.cons a x) :=
+  rfl
+
+def vec_len_non_as : vec n → Nat
+  | vec.nil => 0
+  | vec.cons h t => vec_len_non_as t + 1
+
+def list_len : List Int → Nat
+  | List.nil => 0
+  | x@(List.cons h t) => list_len t + 1
